theories/rules/mem_share.v
@@ -8,47 +8,257 @@ Section mem_share.
 Context `{hypparams: HypervisorParameters}.
 Context `{vmG: !gen_VMG Σ}.
 
-Lemma hvc_mem_share_nz {i wi r0 r1 r2 hvcf p_tx sacc } ai j mem_tx sh (spsd: gset PID) :
+Lemma hvc_mem_share_nz {i wi r0 r1 r2 hvcf p_tx sacc} ai j mem_tx sh (ps: gset PID) :
   (* len is the length of the msg *)
-  let len := (Z.of_nat (finz.to_z r1)) in
+  let len := (Z.to_nat (finz.to_z r1)) in
   (* the decoding of wi is correct *)
   decode_instruction wi = Some(Hvc) ->
-  (* the decoding of R0 is a FFA mem send *)
+  (* the decoding of R0 is a FFA mem_share *)
   decode_hvc_func r0 = Some(hvcf) ->
   hvcf_to_tt hvcf = Some Sharing ->
-  (* caller is not the receiver *)
-  i ≠ j ->
-  (* the descriptor, in list Word *)
-  (* des = serialized_transaction_descriptor i j W0 l (elements spsd) W0 -> *)
   (* the whole descriptor resides in the TX page *)
   (len < page_size)%Z ->
+  (* the descriptor *)
+  parse_transaction_descriptor mem_tx (of_pid p_tx) len = Some (i,None,W0,j,ps) ->
+  (* caller is not the receiver *)
+  i ≠ j ->
+  ps ⊆ sacc ->
   (* there is at least one free handle in the hpool *)
   sh ≠ ∅ ->
   {SS{{ ▷(PC @@ i ->r ai) ∗
       ▷ ai ->a wi ∗
-  (* VM i owns pages in spsd *)
-      ▷ ([∗ set] p ∈ spsd, p -@O> i) ∗
-  (* pages in spsed are exclusive to VM i *)
+      (* VM i exclusively owns pages in ps *)
+      ▷ ([∗ set] p ∈ ps, p -@O> i ∗ p -@E> true) ∗
       ▷ (i -@A> sacc) ∗
-      (* and the page which the instruction is in is not being shared, i.e. (tpa ai) ∉ spsd *)
       ▷ (R0 @@ i ->r r0) ∗
       ▷ (R1 @@ i ->r r1) ∗
       ▷ (R2 @@i ->r r2) ∗
       ▷ (fresh_handles 1 sh) ∗
       ▷ TX@ i := p_tx ∗
-      ▷ mem_region des p_tx
+      ▷ memory_page p_tx mem_tx
        }}}
    ExecI @ i {{{ RET (false,ExecI) ;
                  PC @@ i ->r (ai ^+ 1)%f ∗
                  ai ->a wi ∗
-                 ([∗ set] p ∈ spsd, p -@O> i ) ∗
-                 i -@A> (sacc ∖ spsd) ∗
+                 ([∗ set] p ∈ ps, p -@O> i ) ∗
+                 i -@A> (sacc ∖ ps) ∗
                  R0 @@ i ->r (encode_hvc_ret_code Succ) ∗
                  R1 @@ i ->r r1 ∗
                  (∃ (wh: Word), ⌜wh ∈ sh⌝ ∗
                  R2 @@ i ->r wh ∗
-                 wh ->t (i,W0,j,spsd,Sharing) ∗
+                 wh ->t (i,W0,j,ps,Sharing) ∗
                  wh ->re false ∗
                  fresh_handles 1 (sh∖{[wh]})) ∗
                  TX@ i := p_tx ∗
-                 mem_region des p_tx}}}.
+                 memory_page p_tx mem_tx}}}.
+Proof.
+Admitted.
+
+Lemma hvc_mem_send_invalid_len {i wi r0 r1 r2 hvcf} ai :
+  let len := (Z.to_nat (finz.to_z r1)) in
+  decode_instruction wi = Some(Hvc) ->
+  decode_hvc_func r0 = Some(hvcf) ->
+  ∃ tt, hvcf_to_tt hvcf = Some tt ->
+  (len >= page_size)%Z ->
+  {SS{{ ▷(PC @@ i ->r ai) ∗
+      ▷ ai ->a wi ∗
+      ▷ (R0 @@ i ->r r0) ∗
+      ▷ (R1 @@ i ->r r1) ∗
+      ▷ (R2 @@ i ->r r2)
+       }}}
+   ExecI @ i {{{ RET (false,ExecI) ;
+                 PC @@ i ->r (ai ^+ 1)%f ∗
+                 ai ->a wi ∗
+                 R0 @@ i ->r (encode_hvc_ret_code Error) ∗
+                 R1 @@ i ->r r1 ∗
+                 R2 @@ i ->r (encode_hvc_error InvParam)}}}.
+Proof.
+Admitted.
+
+Lemma hvc_mem_send_invalid_msg {i wi r0 r1 r2 hvcf p_tx} ai mem_tx :
+  let len := (Z.to_nat (finz.to_z r1)) in
+  decode_instruction wi = Some(Hvc) ->
+  decode_hvc_func r0 = Some(hvcf) ->
+  ∃ tt, hvcf_to_tt hvcf = Some tt ->
+  (len < page_size)%Z ->
+  parse_transaction_descriptor mem_tx (of_pid p_tx) len = None ->
+  {SS{{ ▷(PC @@ i ->r ai) ∗
+      ▷ ai ->a wi ∗
+      ▷ (R0 @@ i ->r r0) ∗
+      ▷ (R1 @@ i ->r r1) ∗
+      ▷ (R2 @@ i ->r r2) ∗
+      ▷ (TX@ i := p_tx) ∗
+      ▷ (memory_page p_tx mem_tx)
+       }}}
+   ExecI @ i {{{ RET (false,ExecI) ;
+                 PC @@ i ->r (ai ^+ 1)%f ∗
+                 ai ->a wi ∗
+                 R0 @@ i ->r (encode_hvc_ret_code Error) ∗
+                 R1 @@ i ->r r1 ∗
+                 R2 @@ i ->r (encode_hvc_error InvParam) ∗
+                 TX@ i := p_tx ∗
+                 memory_page p_tx mem_tx
+    }}}.
+Proof.
+Admitted.
+
+Lemma hvc_mem_send_invalid_des {i wi r0 r1 r2 hvcf p_tx tt} ai mem_tx tran :
+  let len := (Z.to_nat (finz.to_z r1)) in
+  decode_instruction wi = Some(Hvc) ->
+  decode_hvc_func r0 = Some(hvcf) ->
+  hvcf_to_tt hvcf = Some tt ->
+  (len < page_size)%Z ->
+  parse_transaction_descriptor mem_tx (of_pid p_tx) len = Some tran ->
+  validate_transaction_descriptor i tt tran = false ->
+  {SS{{ ▷(PC @@ i ->r ai) ∗
+      ▷ ai ->a wi ∗
+      ▷ (R0 @@ i ->r r0) ∗
+      ▷ (R1 @@ i ->r r1) ∗
+      ▷ (R2 @@ i ->r r2) ∗
+      ▷ (TX@ i := p_tx) ∗
+      ▷ (memory_page p_tx mem_tx)
+       }}}
+   ExecI @ i {{{ RET (false,ExecI) ;
+                 PC @@ i ->r (ai ^+ 1)%f ∗
+                 ai ->a wi ∗
+                 R0 @@ i ->r (encode_hvc_ret_code Error) ∗
+                 R1 @@ i ->r r1 ∗
+                 R2 @@ i ->r (encode_hvc_error InvParam) ∗
+                 TX@ i := p_tx ∗
+                 memory_page p_tx mem_tx
+    }}}.
+Proof.
+Admitted.
+
+Lemma hvc_mem_send_not_owned {i wi r0 r1 r2 hvcf p_tx tt} ai mem_tx tran p O :
+  let len := (Z.to_nat (finz.to_z r1)) in
+  decode_instruction wi = Some(Hvc) ->
+  decode_hvc_func r0 = Some(hvcf) ->
+  hvcf_to_tt hvcf = Some tt ->
+  (len < page_size)%Z ->
+  parse_transaction_descriptor mem_tx (of_pid p_tx) len = Some tran ->
+  validate_transaction_descriptor i tt tran = true ->
+  p ∈ tran.2 ->
+  {SS{{ ▷(PC @@ i ->r ai) ∗
+      ▷ ai ->a wi ∗
+      ▷ (R0 @@ i ->r r0) ∗
+      ▷ (R1 @@ i ->r r1) ∗
+      ▷ (R2 @@ i ->r r2) ∗
+      ▷ (TX@ i := p_tx) ∗
+      ▷ (memory_page p_tx mem_tx) ∗
+      ▷ O ∗
+      ▷ (O -∗ (p -@O> - ∨ (∃j, p -@O> j ∗ ⌜j ≠ i⌝)))
+       }}}
+   ExecI @ i {{{ RET (false,ExecI) ;
+                 PC @@ i ->r (ai ^+ 1)%f ∗
+                 ai ->a wi ∗
+                 R0 @@ i ->r (encode_hvc_ret_code Error) ∗
+                 R1 @@ i ->r r1 ∗
+                 R2 @@ i ->r (encode_hvc_error Denied) ∗
+                 TX@ i := p_tx ∗
+                 memory_page p_tx mem_tx ∗
+                 O
+    }}}.
+Proof.
+Admitted.
+
+Lemma hvc_mem_send_not_excl {i wi r0 r1 r2 hvcf p_tx tt} ai mem_tx tran p :
+  let len := (Z.to_nat (finz.to_z r1)) in
+  decode_instruction wi = Some(Hvc) ->
+  decode_hvc_func r0 = Some(hvcf) ->
+  hvcf_to_tt hvcf = Some tt ->
+  (len < page_size)%Z ->
+  parse_transaction_descriptor mem_tx (of_pid p_tx) len = Some tran ->
+  validate_transaction_descriptor i tt tran = true ->
+  p ∈ tran.2 ->
+  {SS{{ ▷(PC @@ i ->r ai) ∗
+      ▷ ai ->a wi ∗
+      ▷ (R0 @@ i ->r r0) ∗
+      ▷ (R1 @@ i ->r r1) ∗
+      ▷ (R2 @@ i ->r r2) ∗
+      ▷ (TX@ i := p_tx) ∗
+      ▷ (memory_page p_tx mem_tx) ∗
+      ▷ (p -@E> false)
+       }}}
+   ExecI @ i {{{ RET (false,ExecI) ;
+                 PC @@ i ->r (ai ^+ 1)%f ∗
+                 ai ->a wi ∗
+                 R0 @@ i ->r (encode_hvc_ret_code Error) ∗
+                 R1 @@ i ->r r1 ∗
+                 R2 @@ i ->r (encode_hvc_error Denied) ∗
+                 TX@ i := p_tx ∗
+                 memory_page p_tx mem_tx ∗
+                 p -@E> false
+    }}}.
+Proof.
+Admitted.
+
+
+Lemma hvc_mem_send_not_acc {i wi r0 r1 r2 hvcf p_tx tt sacc} ai mem_tx tran p :
+  let len := (Z.to_nat (finz.to_z r1)) in
+  decode_instruction wi = Some(Hvc) ->
+  decode_hvc_func r0 = Some(hvcf) ->
+  hvcf_to_tt hvcf = Some tt ->
+  (len < page_size)%Z ->
+  parse_transaction_descriptor mem_tx (of_pid p_tx) len = Some tran ->
+  validate_transaction_descriptor i tt tran = true ->
+  p ∈ tran.2 ->
+  p ∉ sacc ->
+  {SS{{ ▷(PC @@ i ->r ai) ∗
+      ▷ ai ->a wi ∗
+      ▷ (R0 @@ i ->r r0) ∗
+      ▷ (R1 @@ i ->r r1) ∗
+      ▷ (R2 @@ i ->r r2) ∗
+      ▷ (TX@ i := p_tx) ∗
+      ▷ (memory_page p_tx mem_tx) ∗
+      ▷ (i -@A> sacc)
+       }}}
+   ExecI @ i {{{ RET (false,ExecI) ;
+                 PC @@ i ->r (ai ^+ 1)%f ∗
+                 ai ->a wi ∗
+                 R0 @@ i ->r (encode_hvc_ret_code Error) ∗
+                 R1 @@ i ->r r1 ∗
+                 R2 @@ i ->r (encode_hvc_error Denied) ∗
+                 TX@ i := p_tx ∗
+                 memory_page p_tx mem_tx ∗
+                 i -@A> sacc
+    }}}.
+Proof.
+Admitted.
+
+
+Lemma hvc_mem_send_in_trans {i wi r0 r1 r2 hvcf p_tx tt wh q tran'} ai mem_tx tran p :
+  let len := (Z.to_nat (finz.to_z r1)) in
+  decode_instruction wi = Some(Hvc) ->
+  decode_hvc_func r0 = Some(hvcf) ->
+  hvcf_to_tt hvcf = Some tt ->
+  (len < page_size)%Z ->
+  parse_transaction_descriptor mem_tx (of_pid p_tx) len = Some tran ->
+  validate_transaction_descriptor i tt tran = true ->
+  p ∈ tran.2 ->
+  p ∈ tran'.1.2 ->
+  {SS{{ ▷(PC @@ i ->r ai) ∗
+      ▷ ai ->a wi ∗
+      ▷ (R0 @@ i ->r r0) ∗
+      ▷ (R1 @@ i ->r r1) ∗
+      ▷ (R2 @@ i ->r r2) ∗
+      ▷ (TX@ i := p_tx) ∗
+      ▷ (memory_page p_tx mem_tx) ∗
+      ▷ (wh -{q}>t tran')
+       }}}
+   ExecI @ i {{{ RET (false,ExecI) ;
+                 PC @@ i ->r (ai ^+ 1)%f ∗
+                 ai ->a wi ∗
+                 R0 @@ i ->r (encode_hvc_ret_code Error) ∗
+                 R1 @@ i ->r r1 ∗
+                 R2 @@ i ->r (encode_hvc_error Denied) ∗
+                 TX@ i := p_tx ∗
+                 memory_page p_tx mem_tx ∗
+                 wh -{q}>t tran'
+    }}}.
+Proof.
+Admitted.
+
+(* TODO : validate_transaction_descriptor i Sharing tran = true ->
+   ∃ j ps, parse_transaction_descriptor = Some (i,None,W0,j,ps)
+ *)
